lib/Pow.dfy
@@ -1,0 +1,124 @@
+module PowModule {
+
+  function Pow(b: int, e: nat): int {
+    if e == 0 then 1 else b * Pow(b, e - 1)
+  }
+
+  method PowIter(b: int, e: nat) returns (r: int)
+    ensures r == Pow(b, e)
+  {
+    r := 1;
+    var i := 0;
+    while i < e
+      invariant i <= e
+      invariant r == Pow(b, i)
+    {
+      r := r * b;
+      i := i + 1;
+    }
+  }
+
+  lemma Pow0(x: int)
+    ensures Pow(x, 0) == 1
+  {
+  }
+
+  lemma Pow1(x: int)
+    ensures Pow(x, 1) == x
+  {
+  }
+
+  lemma Pow2(x: int)
+    ensures Pow(x, 2) == x * x
+  {
+    assert Pow(x, 2) == x * Pow(x, 1);
+  }
+
+  lemma PowBase0(y: nat)
+    requires y > 0
+    ensures Pow(0, y) == 0
+  {
+  }
+
+  lemma PowMul(x: int, y: int, e: nat)
+    ensures Pow(x * y, e) == Pow(x, e) * Pow(y, e)
+  {
+  }
+
+  lemma PowExpAdd(x: int, a: nat, b: nat)
+    ensures Pow(x, a + b) == Pow(x, a) * Pow(x, b)
+  {
+    if a > 0 {
+      PowExpAdd(x, a - 1, b);
+    }
+  }
+
+  function method FastPow(b: int, e: nat): int
+    decreases e
+  {
+    if e == 0 then 1 
+    else if e % 2 == 0 then FastPow(b * b, e / 2)
+    else b * FastPow(b, e - 1)
+  }
+
+  lemma FastPowEq(b: int, e: nat)
+    ensures FastPow(b, e) == Pow(b, e)
+    decreases e
+  {
+    if e == 0 {
+    } else if e % 2 == 0 {
+      calc {
+        FastPow(b, e);
+        FastPow(b * b, e / 2);
+        { FastPowEq(b * b, e / 2); }
+        Pow(b * b, e / 2);
+        { PowMul(b, b, e / 2); }
+        Pow(b, e / 2) * Pow(b, e / 2);
+        { PowExpAdd(b, e / 2, e / 2); }
+        Pow(b, e / 2 + e / 2);
+      }
+    }
+  }
+
+  method FastPowIter(b: int, e: nat) returns (r: int)
+    ensures r == Pow(b, e)
+  {
+    r := 1;
+    var x := b;
+    var n := e;
+    ghost var ex := 1;
+    ghost var er := 0;
+    while n > 0
+      invariant e == n * ex + er
+      invariant x == Pow(b, ex)
+      invariant r == Pow(b, er)
+    {
+      if n % 2 != 0 {
+        assert r * x == Pow(b, er + ex) by {
+          calc {
+            r * x;
+            Pow(b, er) * Pow(b, ex);
+            { PowExpAdd(b, er, ex); }
+            Pow(b, er + ex);
+          }
+        }
+        r := r * x;
+        n := n - 1;
+        er := er + ex;
+      }
+      assert x * x == Pow(b, ex + ex) by {
+        calc {
+          x * x;
+          Pow(b, ex) * Pow(b, ex);
+          { PowExpAdd(b, ex, ex); }
+          Pow(b, ex + ex);
+        }
+      }
+      assert n % 2 == 0;
+      n := n / 2;
+      x := x * x;
+      ex := ex + ex;
+    }
+  }
+
+}
